IntuitionisticProof contains MinimalProof, so I don't need both. Changed Ni to N.

HOL/IntuitionisticProofScript.sml
@@ -15,47 +15,75 @@ open BagLemmataTheory;
 val _ = new_theory "IntuitionisticProof";
 
 (** Natural Deduction for intuitionistic logic **)
-(* Ni is the 'deduciblility' relation for this system *)
+(* N is the 'deduciblility' relation for this system *)
 (* A, B and C are used to represent formulae *)
 (* D, D1, D2, D3 are used to represent the set of open assumptions *)
 (* I'm representing the deductions simply with unlabeled sets of
    open assumptions, as in T&S 2.1.8-2.1.9 (p.41--44) *)
 
-val (Ni_rules, Ni_ind, Ni_cases) = Hol_reln `
-(! (A :'a formula). Ni {A} A) (* Base case *)
-/\ (!A B D1 D2. (Ni D1 A) /\ (Ni D2 B)
-   ==> (Ni (D1 UNION D2) (A And B))) (* And Intro *)
-/\ (!A B D. (Ni D (A And B)) ==> Ni D A) (* And Elimination Left Conjunct *)
-/\ (!A B D. (Ni D (A And B)) ==> Ni D B) (* And Elim Right Conjunct *)
-/\ (!A B D. (Ni (A INSERT D) B) ==> Ni D (A Imp B)) (* Imp Intro *)
-/\ (!A B D1 D2. (Ni D1 (A Imp B)) /\ (Ni D2 A)
-   ==> Ni (D1 UNION D2) B) (* Imp Elim *)
-/\ (!A B D. Ni D A ==> Ni D (A Or B))  (* Or Intro right *)
-/\ (!A B D. Ni D B ==> Ni D (A Or B))  (* Or Intro left *)
-/\ (!A B C D D1 D2. (Ni D (A Or B)) /\ (* Or Elim *)
-(Ni (A INSERT D1) C) /\ (Ni (B INSERT D2) C) ==> Ni (D ∪ D1 ∪ D2) C)
-/\ (!A D. (Ni D Bot) ==> (Ni D A))`; (* Intuitionistic Absurdity Rule *)
+val (N_rules, N_ind, N_cases) = Hol_reln `
+(! (A :'a formula). N {A} A) (* Base case *)
+/\ (!A B D1 D2. (N D1 A) /\ (N D2 B)
+   ==> (N (D1 UNION D2) (A And B))) (* And Intro *)
+/\ (!A B D. (N D (A And B)) ==> N D A) (* And Elimination Left Conjunct *)
+/\ (!A B D. (N D (A And B)) ==> N D B) (* And Elim Right Conjunct *)
+/\ (!A B D. (N (A INSERT D) B) ==> N D (A Imp B)) (* Imp Intro *)
+/\ (!A B D1 D2. (N D1 (A Imp B)) /\ (N D2 A)
+   ==> N (D1 UNION D2) B) (* Imp Elim *)
+/\ (!A B D. N D A ==> N D (A Or B))  (* Or Intro right *)
+/\ (!A B D. N D B ==> N D (A Or B))  (* Or Intro left *)
+/\ (!A B C D D1 D2. (N D (A Or B)) /\ (* Or Elim *)
+(N (A INSERT D1) C) /\ (N (B INSERT D2) C) ==> N (D ∪ D1 ∪ D2) C)
+/\ (!A D. (N D Bot) ==> (N D A))`; (* Intuitionistic Absurdity Rule *)
 
-val [Ni_ax, Ni_andi, Ni_andel, Ni_ander,
-     Ni_impi, Ni_impe, Ni_orir, Ni_oril, Ni_ore, Ni_bot] = CONJUNCTS Ni_rules;
+val [N_ax, N_andi, N_andel, N_ander,
+     N_impi, N_impe, N_orir, N_oril, N_ore, N_bot] = CONJUNCTS N_rules;
 
-Theorem Ni_FINITE:
-  !D A. Ni D A ==> FINITE D
-Proof Induct_on `Ni` >> rw[]
+Theorem N_FINITE:
+  !D A. N D A ==> FINITE D
+Proof Induct_on `N` >> rw[]
 QED
 
-Theorem Ni_lw:
-  ∀D A. Ni D A ==> ∀B. Ni (B INSERT D) A
+val (Nd_rules, Nd_ind, Nd_cases) = Hol_reln `
+(! (A :'a formula). Nd {A} A) (* Base case *)
+/\ (!A B D1 D2. (Nd D1 A) /\ (Nd D2 B)
+    ==> (Nd (D1 UNION D2) (A And B))) (* And Intro *)
+/\ (!A B D. (Nd D (A And B)) ==> Nd D A) (* And Elimination Left Conjunct *)
+/\ (!A B D. (Nd D (A And B)) ==> Nd D B) (* And Elim Right Conjunct *)
+/\ (!A B D. (Nd D B) ==> Nd (D DELETE A) (A Imp B)) (* Imp Intro *)
+/\ (!A B D1 D2. (Nd D1 (A Imp B)) /\ (Nd D2 A)
+    ==> Nd (D1 UNION D2) B) (* Imp Elim *)
+/\ (!A B D. Nd D A ==> Nd D (A Or B)) (* Or Intro right *)
+/\ (!A B D. Nd D B ==> Nd D (A Or B)) (* Or Intro left *)
+/\ (!A B C D D1 D2. (Nd D (A Or B)) /\ (Nd D1 C) /\ (Nd D2 C)
+    ==> Nd (D ∪ (D1 DELETE A) ∪ (D2 DELETE B)) C) (* Or Elim *)
+/\ (!A D. (Nd D Bot) ==> (Nd D A))`; (* Intuitionistic Absurdity Rule *)
+
+val [Nd_ax, Nd_andi, Nd_andel, Nd_ander,
+     Nd_impi, Nd_impe, Nd_orir, Nd_oril, Nd_ore, Nd_bot] = CONJUNCTS Nd_rules;
+
+Theorem N_lw:
+  ∀D A. N D A ==> ∀B. N (B INSERT D) A
 Proof
   rw[] >>
-  `Ni {B} B` by metis_tac[Ni_ax] >>
-  `Ni ({B} ∪ D) (B And A)` by metis_tac[Ni_andi] >>
-  `Ni ({B} ∪ D) A` by metis_tac[Ni_ander] >>
+  `N {B} B` by metis_tac[N_ax] >>
+  `N ({B} ∪ D) (B And A)` by metis_tac[N_andi] >>
+  `N ({B} ∪ D) A` by metis_tac[N_ander] >>
   metis_tac[INSERT_SING_UNION]
 QED
 
-Theorem Ni_lw_SUBSET:
-  ∀D'. FINITE D' ==> ∀D A. Ni D A  /\ D ⊆ D' ==> Ni D' A
+Theorem Nd_lw:
+∀D A. Nd D A ==> ∀B. Nd (B INSERT D) A
+Proof
+  rw[] >>
+  `Nd {B} B` by metis_tac[Nd_ax] >>
+  `Nd ({B} ∪ D) (B And A)` by metis_tac[Nd_andi] >>
+  `Nd ({B} ∪ D) A` by metis_tac[Nd_ander] >>
+  metis_tac[INSERT_SING_UNION]
+QED
+
+Theorem N_lw_SUBSET:
+  ∀D'. FINITE D' ==> ∀D A. N D A  /\ D ⊆ D' ==> N D' A
 Proof
   GEN_TAC >>
   Induct_on `CARD D'`
@@ -73,14 +101,33 @@ Proof
             fs[SUBSET_DEF]) >>
           rw[] >>
           fs[] >>
-          metis_tac[Ni_lw]))
+          metis_tac[N_lw]))
 QED
 
-Theorem Ni_impi_DELETE:
-  ∀D A B. Ni D A ==> Ni (D DELETE B) (B Imp A)
+Theorem Nd_lw_SUBSET:
+∀D'. FINITE D' ==> ∀D A. Nd D A  /\ D ⊆ D' ==> Nd D' A
+Proof
+  GEN_TAC >>
+  Induct_on `CARD D'`
+  >- (rw[] >> metis_tac[CARD_EQ_0,SUBSET_EMPTY])
+  >- (rw[] >> Cases_on `D=D'` >- metis_tac[] >>
+      `?D₀ e. (D' = e INSERT D₀) /\ D ⊆ D₀ /\ e NOTIN D₀`
+        by (`?e. e ∈ D' /\ e NOTIN D`
+              by metis_tac[PSUBSET_DEF,PSUBSET_MEMBER] >>
+            qexists_tac `D' DELETE e` >>
+            qexists_tac `e` >>
+            simp[] >>
+            fs[SUBSET_DEF]) >>
+      rw[] >>
+      fs[] >>
+      metis_tac[Nd_lw])
+QED
+
+Theorem N_impi_DELETE:
+  ∀D A B. N D A ==> N (D DELETE B) (B Imp A)
 Proof
   rw[] >>
-  `Ni (B INSERT D) A` by metis_tac[Ni_lw] >>
+  `N (B INSERT D) A` by metis_tac[N_lw] >>
   Cases_on `B ∈ D`
     >- (`?D'. (D = B INSERT D') /\ B NOTIN D'`
           by metis_tac[DECOMPOSITION] >>
@@ -88,190 +135,240 @@ Proof
         `(B INSERT D') DELETE B = D'`
           by (dsimp[EXTENSION] >>
               metis_tac[]) >>
-        simp[Ni_impi])
-    >- simp[DELETE_NON_ELEMENT_RWT,Ni_impi]
+        simp[N_impi])
+    >- simp[DELETE_NON_ELEMENT_RWT,N_impi]
 QED
 
-val NiThm = Define `NiThm A = Ni EMPTY A`;
+Theorem N_Nd:
+  ∀D A. N D A <=> Nd D A
+Proof
+ `(∀D A:'a formula. N D A ==> Nd D A) ∧
+  (∀D A:'a formula. Nd D A ==> N D A)`
+    suffices_by metis_tac[] >>
+  conj_tac
+  >- (Induct_on `N` >>
+      rw[Nd_rules]
+        >- metis_tac[Nd_andel]
+        >- metis_tac[Nd_ander]
+        >- (`Nd ((A INSERT D) DELETE A) (A Imp B)`
+              by metis_tac[Nd_impi] >>
+            Cases_on `A ∈ D`
+              >- (fs[DELETE_DEF] >>
+                  `Nd (A INSERT (D DIFF {A})) (A Imp B)`
+                    by metis_tac[Nd_lw] >>
+                  fs[Once INSERT_SING_UNION] >>
+                  `{A} ⊆ D` by simp[SUBSET_DEF] >>
+                  metis_tac[UNION_DIFF])
+              >- fs[DELETE_DEF,DELETE_NON_ELEMENT])
+        >- metis_tac[Nd_impe]
+        >- (`Nd (D ∪ ((A INSERT D1) DELETE A) ∪ ((B INSERT D2) DELETE B)) C`
+              by metis_tac[Nd_ore] >>
+            fs[DELETE_DEF] >>
+            irule Nd_lw_SUBSET >>
+            `FINITE (D ∪ D1 ∪ D2)`
+              by (simp[FINITE_UNION] >> metis_tac[N_FINITE,FINITE_INSERT]) >>
+            simp[] >>
+            qexists_tac `D ∪ (D1 DIFF {A}) ∪ (D2 DIFF {B})` >>
+            rw[SUBSET_DEF]))
+  >- (Induct_on `Nd` >>
+      rw[N_rules]
+        >- metis_tac[N_andel]
+        >- metis_tac[N_ander]
+        >- metis_tac[N_impi_DELETE]
+        >- metis_tac[N_impe]
+        >- (`N (A INSERT (D1 DELETE A)) C`
+              by (irule N_lw_SUBSET >>
+                  rw[] >- metis_tac[N_FINITE] >>
+                  qexists_tac `D1` >>
+                  rw[DELETE_DEF,SUBSET_DEF]) >>
+            `N (B INSERT (D2 DELETE B)) C`
+              by (irule N_lw_SUBSET >>
+                  rw[] >- metis_tac[N_FINITE] >>
+                  qexists_tac `D2` >>
+                  rw[DELETE_DEF,SUBSET_DEF]) >>
+            metis_tac[N_ore]))
+QED
+
+val NThm = Define `NThm A = N EMPTY A`;
 
 (* Example deductions *)
-val Ni_example = Q.prove(`NiThm (A Imp (B Imp A))`,
-`Ni {A} A` by rw[Ni_ax] >>
-`Ni {B} B` by rw[Ni_ax] >>
+val N_example = Q.prove(`NThm (A Imp (B Imp A))`,
+`N {A} A` by rw[N_ax] >>
+`N {B} B` by rw[N_ax] >>
 `{A} UNION {B} = {A;B}` by simp[UNION_DEF,INSERT_DEF] >>
-`Ni {A;B} (A And B)` by metis_tac[Ni_andi] >>
-`Ni {A;B} (A)` by metis_tac[Ni_andel] >>
-`Ni {A} (B Imp A)` by (irule Ni_impi >> simp[INSERT_COMM]) >>
-`Ni {} (A Imp (B Imp A))` by metis_tac[Ni_impi] >>
- rw[NiThm]);
+`N {A;B} (A And B)` by metis_tac[N_andi] >>
+`N {A;B} (A)` by metis_tac[N_andel] >>
+`N {A} (B Imp A)` by (irule N_impi >> simp[INSERT_COMM]) >>
+`N {} (A Imp (B Imp A))` by metis_tac[N_impi] >>
+ rw[NThm]);
 
-val Ni_example = Q.prove(`NiThm (Bot Imp A)`,
-  `Ni {Bot} Bot` by rw[Ni_rules] >>
-  `Ni {Bot} A` by rw[Ni_rules] >>
+val N_example = Q.prove(`NThm (Bot Imp A)`,
+  `N {Bot} Bot` by rw[N_rules] >>
+  `N {Bot} A` by rw[N_rules] >>
   `{} = ({Bot} DIFF {Bot})` by rw[DIFF_DEF] >>
-  `Ni EMPTY (Bot Imp A)` by metis_tac[Ni_rules] >>
-  rw[NiThm]);
+  `N EMPTY (Bot Imp A)` by metis_tac[N_rules] >>
+  rw[NThm]);
 
 
 (** Sequent Calculus (Gentzen System) for intuitionistic logic **)
-(* Gi is the 'deduciblility' relation for this system *)
+(* G is the 'deduciblility' relation for this system *)
 (* A, B and C are used to represent formulae *)
 (* S is used to represent the multiset of the Antecedent Context *)
 (* The consequent is always a single formula in the intuitionistic logic *)
 
-val (Gi_rules, Gi_ind, Gi_cases) = Hol_reln `
-(!(A:'a formula) Γ. (A <: Γ) /\ FINITE_BAG Γ ==> Gi Γ A) (* Ax *)
-/\ (∀ A Γ. (Bot <: Γ) /\ FINITE_BAG Γ ==> Gi Γ A) (* LBot *)
-/\ (!A Γ C. (Gi ({|A;A|} + Γ) C)
-   ==> Gi ({|A|} + Γ) C) (* Left Contraction *)
-/\ (!A B Γ C. (Gi (BAG_INSERT A Γ) C)
-   ==> (Gi (BAG_INSERT (A And B) Γ) C)) (* Left And 1 *)
-/\ (!A B Γ C. (Gi (BAG_INSERT B Γ) C)
-   ==> (Gi (BAG_INSERT (A And B) Γ) C)) (* Left And 2 *)
-/\ (!A B Γ. (Gi Γ A) /\ (Gi Γ B)
-   ==> (Gi Γ (A And B))) (* Right And *)
-/\ (!A B Γ C. (Gi (BAG_INSERT A Γ) C)
-    /\ (Gi (BAG_INSERT B Γ) C)
-   ==> (Gi (BAG_INSERT (A Or B) Γ) C)) (* Left Or *)
-/\ (!A B Γ. (Gi Γ A)
-   ==> (Gi Γ (A Or B))) (* Right Or 1 *)
-/\ (!A B Γ. (Gi Γ B)
-   ==> (Gi Γ (A Or B))) (* Right Or 2 *)
-/\ (!A B Γ C. (Gi Γ A) /\ (Gi (BAG_INSERT B Γ) C)
-   ==> (Gi (BAG_INSERT (A Imp B) Γ) C)) (* Left Imp *)
-/\ (!A B Γ. (Gi (BAG_INSERT A Γ) B)
-   ==> (Gi Γ (A Imp B))) (* Right Imp *)
-∧  (∀A B Γ Δ. (Gi Γ A) ∧ (Gi (BAG_INSERT A Δ) B) ==> Gi (Γ + Δ) B)` (* Cut *)
+val (G_rules, G_ind, G_cases) = Hol_reln `
+(!(A:'a formula) Γ. (A <: Γ) /\ FINITE_BAG Γ ==> G Γ A) (* Ax *)
+/\ (∀ A Γ. (Bot <: Γ) /\ FINITE_BAG Γ ==> G Γ A) (* LBot *)
+/\ (!A Γ C. (G ({|A;A|} + Γ) C)
+   ==> G ({|A|} + Γ) C) (* Left Contraction *)
+/\ (!A B Γ C. (G (BAG_INSERT A Γ) C)
+   ==> (G (BAG_INSERT (A And B) Γ) C)) (* Left And 1 *)
+/\ (!A B Γ C. (G (BAG_INSERT B Γ) C)
+   ==> (G (BAG_INSERT (A And B) Γ) C)) (* Left And 2 *)
+/\ (!A B Γ. (G Γ A) /\ (G Γ B)
+   ==> (G Γ (A And B))) (* Right And *)
+/\ (!A B Γ C. (G (BAG_INSERT A Γ) C)
+    /\ (G (BAG_INSERT B Γ) C)
+   ==> (G (BAG_INSERT (A Or B) Γ) C)) (* Left Or *)
+/\ (!A B Γ. (G Γ A)
+   ==> (G Γ (A Or B))) (* Right Or 1 *)
+/\ (!A B Γ. (G Γ B)
+   ==> (G Γ (A Or B))) (* Right Or 2 *)
+/\ (!A B Γ C. (G Γ A) /\ (G (BAG_INSERT B Γ) C)
+   ==> (G (BAG_INSERT (A Imp B) Γ) C)) (* Left Imp *)
+/\ (!A B Γ. (G (BAG_INSERT A Γ) B)
+   ==> (G Γ (A Imp B))) (* Right Imp *)
+∧  (∀A B Γ Δ. (G Γ A) ∧ (G (BAG_INSERT A Δ) B) ==> G (Γ + Δ) B)` (* Cut *)
 
-val [Gi_ax, Gi_bot, Gi_lc, Gi_landl, Gi_landr, Gi_rand,
-     Gi_lor, Gi_rorl, Gi_rorr, Gi_limp, Gi_rimp, Gi_cut] = CONJUNCTS Gi_rules;
+val [G_ax, G_bot, G_lc, G_landl, G_landr, G_rand,
+     G_lor, G_rorl, G_rorr, G_limp, G_rimp, G_cut] = CONJUNCTS G_rules;
 
-val GiThm = Define `GiThm A = Gi EMPTY_BAG A`;
+val GThm = Define `GThm A = G EMPTY_BAG A`;
 
-val Gi_example1 =
-    Q.prove(`GiThm ((A And B) Imp (B And A))`, rw[GiThm,Gi_rules]);
+val G_example1 =
+    Q.prove(`GThm ((A And B) Imp (B And A))`, rw[GThm,G_rules]);
 
-val Gi_example2 = Q.prove (`GiThm ((A Imp (A Imp B)) Imp (A Imp B))`,
-rw[GiThm] >>
-`Gi {|(A Imp A Imp B)|} (A Imp B)` suffices_by metis_tac[Gi_rules] >>
-`Gi {|A;(A Imp A Imp B)|} (B)` suffices_by metis_tac[Gi_rules] >>
-`Gi {|A|} (A)` by metis_tac[Gi_ax,BAG_IN_BAG_INSERT,FINITE_BAG] >>
-`Gi {|B;A|} (B)` by metis_tac[Gi_ax,BAG_IN_BAG_INSERT,FINITE_BAG] >>
-(* `Gi {|A;B|} (B)` by simp[Gi_lw] >> *)
-(* `Gi {|B;A|} (B)` by simp[BAG_INSERT_commutes] >> *)
-`Gi {|(A Imp B);A|} (B)` by metis_tac[Gi_rules] >>
-`Gi {|(A Imp A Imp B);A|} (B)` suffices_by metis_tac[BAG_INSERT_commutes] >>
-metis_tac[Gi_rules]);
+val G_example2 = Q.prove (`GThm ((A Imp (A Imp B)) Imp (A Imp B))`,
+rw[GThm] >>
+`G {|(A Imp A Imp B)|} (A Imp B)` suffices_by metis_tac[G_rules] >>
+`G {|A;(A Imp A Imp B)|} (B)` suffices_by metis_tac[G_rules] >>
+`G {|A|} (A)` by metis_tac[G_ax,BAG_IN_BAG_INSERT,FINITE_BAG] >>
+`G {|B;A|} (B)` by metis_tac[G_ax,BAG_IN_BAG_INSERT,FINITE_BAG] >>
+(* `G {|A;B|} (B)` by simp[G_lw] >> *)
+(* `G {|B;A|} (B)` by simp[BAG_INSERT_commutes] >> *)
+`G {|(A Imp B);A|} (B)` by metis_tac[G_rules] >>
+`G {|(A Imp A Imp B);A|} (B)` suffices_by metis_tac[BAG_INSERT_commutes] >>
+metis_tac[G_rules]);
 
-val Gi_land_commutes =
-    Q.prove(`Gi {| A And B |} Δ ==> Gi {| B And A |} Δ`, rw[] >>
-`Gi {|B|} B` by metis_tac[Gi_ax,BAG_IN_BAG_INSERT,FINITE_BAG] >>
-`Gi {|B And A|} B` by metis_tac[Gi_landl] >>
-`Gi {|A|} A` by metis_tac[Gi_ax,BAG_IN_BAG_INSERT,FINITE_BAG] >>
-`Gi {|B And A|} A` by metis_tac[Gi_landr] >>
-`Gi {|B And A|} (A And B)` by metis_tac[Gi_rand] >>
-`Gi ({|B And A|} + {||}) Δ` by metis_tac[Gi_cut] >>
+val G_land_commutes =
+    Q.prove(`G {| A And B |} Δ ==> G {| B And A |} Δ`, rw[] >>
+`G {|B|} B` by metis_tac[G_ax,BAG_IN_BAG_INSERT,FINITE_BAG] >>
+`G {|B And A|} B` by metis_tac[G_landl] >>
+`G {|A|} A` by metis_tac[G_ax,BAG_IN_BAG_INSERT,FINITE_BAG] >>
+`G {|B And A|} A` by metis_tac[G_landr] >>
+`G {|B And A|} (A And B)` by metis_tac[G_rand] >>
+`G ({|B And A|} + {||}) Δ` by metis_tac[G_cut] >>
 metis_tac[BAG_UNION_EMPTY]);
 
-Theorem Gi_FINITE:
-  !D A. Gi D A ==> FINITE_BAG D
-Proof Induct_on `Gi` >> rw[]
+Theorem G_FINITE:
+  !D A. G D A ==> FINITE_BAG D
+Proof Induct_on `G` >> rw[]
 QED
 
 (* Thanks for this theorem Michael *)
-Theorem Gi_lw:
-  ∀Γ A. Gi Γ A ⇒ ∀Γ'. Γ ≤ Γ' /\ FINITE_BAG Γ' ⇒ Gi Γ' A
+Theorem G_lw:
+  ∀Γ A. G Γ A ⇒ ∀Γ'. Γ ≤ Γ' /\ FINITE_BAG Γ' ⇒ G Γ' A
 Proof
-  Induct_on `Gi` >> rw[]
-  >- (irule Gi_ax >> fs[SUB_BAG, BAG_IN])
-  >- (irule Gi_bot >> fs[SUB_BAG,BAG_IN])
+  Induct_on `G` >> rw[]
+  >- (irule G_ax >> fs[SUB_BAG, BAG_IN])
+  >- (irule G_bot >> fs[SUB_BAG,BAG_IN])
   >- (‘∃Γ₂. Γ' = {|A|} ⊎ Γ₂’
         by (qexists_tac ‘Γ' - {|A|}’ >> irule SUB_BAG_DIFF_EQ >>
             metis_tac[SUB_BAG_UNION_down]) >>
-      rw[] >> irule Gi_lc >> first_x_assum irule >> simp[] >> fs[])
+      rw[] >> irule G_lc >> first_x_assum irule >> simp[] >> fs[])
   >- (‘∃Γ₂. Γ' = BAG_INSERT (A And B) Γ₂’
         by (qexists_tac ‘Γ' - {|A And B|}’ >> fs[BAG_INSERT_UNION] >>
             irule SUB_BAG_DIFF_EQ >> metis_tac[SUB_BAG_UNION_down]) >>
-      rw[] >> irule Gi_landl >> first_x_assum irule >> fs[SUB_BAG_INSERT])
+      rw[] >> irule G_landl >> first_x_assum irule >> fs[SUB_BAG_INSERT])
   >- (‘∃Γ₂. Γ' = BAG_INSERT (A And B) Γ₂’
         by (qexists_tac ‘Γ' - {|A And B|}’ >> fs[BAG_INSERT_UNION] >>
             irule SUB_BAG_DIFF_EQ >> metis_tac[SUB_BAG_UNION_down]) >>
-      rw[] >> irule Gi_landr >> first_x_assum irule >> fs[SUB_BAG_INSERT])
-  >- (irule Gi_rand >> simp[])
+      rw[] >> irule G_landr >> first_x_assum irule >> fs[SUB_BAG_INSERT])
+  >- (irule G_rand >> simp[])
   >- (‘∃Γ₂. Γ' = BAG_INSERT (A Or B) Γ₂’
         by (qexists_tac ‘Γ' - {|A Or B|}’ >> fs[BAG_INSERT_UNION] >>
             irule SUB_BAG_DIFF_EQ >> metis_tac[SUB_BAG_UNION_down]) >>
-      rw[] >> fs[SUB_BAG_INSERT] >> irule Gi_lor >> conj_tac >>
+      rw[] >> fs[SUB_BAG_INSERT] >> irule G_lor >> conj_tac >>
       first_x_assum (fn th => irule th >> fs[SUB_BAG_INSERT] >> NO_TAC))
-  >- simp[Gi_rorl]
-  >- simp[Gi_rorr]
+  >- simp[G_rorl]
+  >- simp[G_rorr]
   >- (‘∃Γ₂. Γ' = BAG_INSERT (A Imp B) Γ₂’
         by (qexists_tac ‘Γ' - {|A Imp B|}’ >> fs[BAG_INSERT_UNION] >>
             irule SUB_BAG_DIFF_EQ >> metis_tac[SUB_BAG_UNION_down]) >>
-      rw[] >> irule Gi_limp >> fs[SUB_BAG_INSERT])
-  >- simp[SUB_BAG_INSERT, Gi_rimp]
+      rw[] >> irule G_limp >> fs[SUB_BAG_INSERT])
+  >- simp[SUB_BAG_INSERT, G_rimp]
   >- (rename [‘Γ₁ ⊎ Γ₂ ≤ Γ₃’] >>
       ‘∃Γ₀. Γ₃ = Γ₀ ⊎ Γ₁ ⊎ Γ₂’
         by metis_tac[SUB_BAG_EXISTS, COMM_BAG_UNION, ASSOC_BAG_UNION] >>
-      rw[] >> irule Gi_cut >>
-      rename [‘Gi (BAG_INSERT A _) B’] >> qexists_tac ‘A’ >>
+      rw[] >> irule G_cut >>
+      rename [‘G (BAG_INSERT A _) B’] >> qexists_tac ‘A’ >>
       conj_tac >> first_x_assum irule >> fs[SUB_BAG_INSERT])
 QED
 
-Theorem Gi_lw_BAG_MERGE:
-  !Γ₁ A. Gi Γ₁ A ==> !Γ₂. FINITE_BAG Γ₂ ==> Gi (BAG_MERGE Γ₂ Γ₁) A
+Theorem G_lw_BAG_MERGE:
+  !Γ₁ A. G Γ₁ A ==> !Γ₂. FINITE_BAG Γ₂ ==> G (BAG_MERGE Γ₂ Γ₁) A
 Proof
   rw[] >>
-  irule Gi_lw >>
-  `FINITE_BAG Γ₁` by metis_tac[Gi_FINITE] >>
+  irule G_lw >>
+  `FINITE_BAG Γ₁` by metis_tac[G_FINITE] >>
   simp[FINITE_BAG_MERGE] >>
   qexists_tac `Γ₁` >>
   simp[SUB_BAG,BAG_INN_BAG_MERGE]
 QED
 
-Theorem Gi_lw_BAG_UNION:
-  ∀Γ A. Gi Γ A ==> ∀Γ'. FINITE_BAG Γ' ==> Gi (Γ ⊎ Γ') A
+Theorem G_lw_BAG_UNION:
+  ∀Γ A. G Γ A ==> ∀Γ'. FINITE_BAG Γ' ==> G (Γ ⊎ Γ') A
 Proof
   rw[] >>
-  irule Gi_lw >>
-  `FINITE_BAG Γ` by metis_tac[Gi_FINITE] >>
+  irule G_lw >>
+  `FINITE_BAG Γ` by metis_tac[G_FINITE] >>
   simp[FINITE_BAG_UNION] >>
   qexists_tac `Γ` >>
   simp[]
 QED
 
-Theorem Gi_lw_BAG_INSERT:
-  ∀Γ A. Gi Γ A ==> ∀B Γ'. Gi (BAG_INSERT B Γ) A
+Theorem G_lw_BAG_INSERT:
+  ∀Γ A. G Γ A ==> ∀B Γ'. G (BAG_INSERT B Γ) A
 Proof
   rw[] >>
-  irule Gi_lw >>
-  `FINITE_BAG Γ` by metis_tac[Gi_FINITE] >>
+  irule G_lw >>
+  `FINITE_BAG Γ` by metis_tac[G_FINITE] >>
   simp[FINITE_BAG_THM] >>
   qexists_tac `Γ` >>
   simp[SUB_BAG_INSERT_I]
 QED
 
-val Gi_lc_AeA =
-    Q.prove(`∀A e Γ'. Gi (BAG_INSERT A (BAG_INSERT e (BAG_INSERT A Γ'))) B
-            ==> Gi (BAG_INSERT e (BAG_INSERT A Γ')) B`,
+val G_lc_AeA =
+    Q.prove(`∀A e Γ'. G (BAG_INSERT A (BAG_INSERT e (BAG_INSERT A Γ'))) B
+            ==> G (BAG_INSERT e (BAG_INSERT A Γ')) B`,
             rw[] >>
-            `Gi ({|A;A|} ⊎ ({|e|} ⊎ Γ')) B`
+            `G ({|A;A|} ⊎ ({|e|} ⊎ Γ')) B`
               by (fs[BAG_UNION_INSERT,ASSOC_BAG_UNION,BAG_INSERT_UNION] >>
                   simp[COMM_BAG_UNION] >>
                   fs[EL_BAG,BAG_UNION]) >>
-            `Gi ({|A|} ⊎ ({|e|} ⊎ Γ')) B`
-              by metis_tac[Gi_lc] >>
-            `Gi (({|A|} ⊎ {|e|}) ⊎ Γ') B`
+            `G ({|A|} ⊎ ({|e|} ⊎ Γ')) B`
+              by metis_tac[G_lc] >>
+            `G (({|A|} ⊎ {|e|}) ⊎ Γ') B`
               by fs[ASSOC_BAG_UNION] >>
-            `Gi (({|e|} ⊎ {|A|}) ⊎ Γ') B`
+            `G (({|e|} ⊎ {|A|}) ⊎ Γ') B`
               by fs[COMM_BAG_UNION] >>
             fs[BAG_INSERT_UNION] >>
             fs[EL_BAG] >>
             simp[ASSOC_BAG_UNION]);
 
-Theorem Gi_INSERT_TO_MERGE:
+Theorem G_INSERT_TO_MERGE:
   ∀Γ. FINITE_BAG Γ ==>
-      ∀A B. Gi (BAG_INSERT A Γ) B ==> Gi (BAG_MERGE {|A|} Γ) B
+      ∀A B. G (BAG_INSERT A Γ) B ==> G (BAG_MERGE {|A|} Γ) B
 Proof
     Induct_on `Γ` >>
     rw[] >>
@@ -281,17 +378,17 @@ Proof
             by (simp[BAG_MERGE,BAG_INSERT,EMPTY_BAG,FUN_EQ_THM] >>
                 rw[] >> fs[]) >>
           fs[] >>
-          `Gi ({|e;e|} ⊎ Γ) B` by fs[BAG_INSERT_UNION,ASSOC_BAG_UNION] >>
-          `Gi ({|e|} ⊎ Γ) B` by metis_tac[Gi_lc] >>
+          `G ({|e;e|} ⊎ Γ) B` by fs[BAG_INSERT_UNION,ASSOC_BAG_UNION] >>
+          `G ({|e|} ⊎ Γ) B` by metis_tac[G_lc] >>
           `{|e|} ⊎ Γ = BAG_INSERT e Γ`
             by rw[BAG_INSERT_UNION] >>
           metis_tac[])
       >- (Cases_on `BAG_IN A Γ`
           >- (`?Γ'. Γ = BAG_INSERT A Γ'` by metis_tac[BAG_DECOMPOSE] >>
               fs[] >>
-              `Gi (BAG_INSERT e (BAG_INSERT A Γ')) B`
-                by metis_tac[Gi_lc_AeA] >>
-              fs[Gi_lw_BAG_MERGE])
+              `G (BAG_INSERT e (BAG_INSERT A Γ')) B`
+                by metis_tac[G_lc_AeA] >>
+              fs[G_lw_BAG_MERGE])
           >- (`BAG_INSERT A (BAG_INSERT e Γ)
                 = BAG_MERGE {|A|} (BAG_INSERT e Γ)`
                 by (`Γ A = 0` by metis_tac[NOT_BAG_IN] >>
@@ -304,12 +401,12 @@ QED
 val unibag_AA_A = Q.prove(`unibag ({|A;A|} ⊎ Γ) = unibag ({|A|} ⊎ Γ)`,
   simp[unibag_thm]);
 
-Theorem Gi_unibag:
-  ∀Γ A. Gi Γ A <=> Gi (unibag Γ) A
+Theorem G_unibag:
+  ∀Γ A. G Γ A <=> G (unibag Γ) A
 Proof
   rw[] >> EQ_TAC
-  >- (`∀Γ. FINITE_BAG Γ ==> ∀A. Gi Γ A ==> Gi (unibag Γ) A`
-        suffices_by metis_tac[Gi_FINITE] >>
+  >- (`∀Γ. FINITE_BAG Γ ==> ∀A. G Γ A ==> G (unibag Γ) A`
+        suffices_by metis_tac[G_FINITE] >>
       gen_tac >>
       Induct_on `BAG_CARD Γ` >>
       rw[]
@@ -318,63 +415,63 @@ Proof
         >- (Cases_on `unibag Γ = Γ` >- fs[] >>
             drule_then strip_assume_tac unibag_DECOMPOSE >>
             rename [`Γ = {|B;B|} ⊎ Γ0`,`SUC n = BAG_CARD Γ`] >>
-            `Gi ({|B|} ⊎ Γ0) A` by metis_tac[Gi_lc] >>
+            `G ({|B|} ⊎ Γ0) A` by metis_tac[G_lc] >>
             `BAG_CARD ({|B|} ⊎ Γ0) = n` by fs[BAG_CARD_THM] >>
             `FINITE_BAG ({|B|} ⊎ Γ0)` by fs[] >>
             metis_tac[unibag_AA_A]))
-   >- metis_tac[unibag_SUB_BAG,Gi_lw,Gi_FINITE,unibag_FINITE]
+   >- metis_tac[unibag_SUB_BAG,G_lw,G_FINITE,unibag_FINITE]
 QED
 
-Theorem Ni_Gi:
-  ∀Γ A. Ni Γ A ==> Gi (BAG_OF_SET Γ) A
+Theorem N_G:
+  ∀Γ A. N Γ A ==> G (BAG_OF_SET Γ) A
 Proof
- Induct_on `Ni ` >>
- rw[Gi_rules]
- (* >- (irule Gi_ax >> simp[] >> *)
+ Induct_on `N ` >>
+ rw[G_rules]
+ (* >- (irule G_ax >> simp[] >> *)
  (*     metis_tac[FINITE_BAG_OF_SET,FINITE_DEF]) *)
- >- (irule Gi_rand >> conj_tac
-     >- (`Gi (BAG_OF_SET (Γ' ∪ Γ)) A` suffices_by metis_tac[UNION_COMM] >>
+ >- (irule G_rand >> conj_tac
+     >- (`G (BAG_OF_SET (Γ' ∪ Γ)) A` suffices_by metis_tac[UNION_COMM] >>
          simp[BAG_OF_SET_UNION] >>
-         metis_tac[Gi_lw_BAG_MERGE,Gi_FINITE])
+         metis_tac[G_lw_BAG_MERGE,G_FINITE])
      >- (simp[BAG_OF_SET_UNION] >>
-             metis_tac[Gi_lw_BAG_MERGE,Gi_FINITE]))
- >- (`Gi {|A|} A` by metis_tac[Gi_ax,BAG_IN_BAG_INSERT,FINITE_BAG] >>
-     `Gi {|A And B|} A` by metis_tac[Gi_landl] >>
-     `Gi ((BAG_OF_SET Γ) + {||}) A` by metis_tac[Gi_cut] >>
+             metis_tac[G_lw_BAG_MERGE,G_FINITE]))
+ >- (`G {|A|} A` by metis_tac[G_ax,BAG_IN_BAG_INSERT,FINITE_BAG] >>
+     `G {|A And B|} A` by metis_tac[G_landl] >>
+     `G ((BAG_OF_SET Γ) + {||}) A` by metis_tac[G_cut] >>
      metis_tac[BAG_UNION_EMPTY])
- >- (`Gi {|A'|} A'` by metis_tac[Gi_ax,BAG_IN_BAG_INSERT,FINITE_BAG] >>
-     `Gi {|A And A'|} A'` by metis_tac[Gi_landr] >>
-     `Gi ((BAG_OF_SET Γ) + {||}) A'` by metis_tac[Gi_cut] >>
+ >- (`G {|A'|} A'` by metis_tac[G_ax,BAG_IN_BAG_INSERT,FINITE_BAG] >>
+     `G {|A And A'|} A'` by metis_tac[G_landr] >>
+     `G ((BAG_OF_SET Γ) + {||}) A'` by metis_tac[G_cut] >>
      metis_tac[BAG_UNION_EMPTY])
- >- (irule Gi_rimp >>
+ >- (irule G_rimp >>
      fs[BAG_OF_SET_INSERT] >>
-     irule Gi_lw >>
+     irule G_lw >>
      simp[] >>
-     drule Gi_FINITE >>
+     drule G_FINITE >>
      rw[] >>
      qexists_tac `BAG_MERGE {|A|} (BAG_OF_SET Γ)` >>
      simp[BAG_MERGE_ELBAG_SUB_BAG_INSERT])
  >- (simp[BAG_OF_SET_UNION] >>
-    `FINITE_BAG (BAG_OF_SET Γ')` by metis_tac[Ni_FINITE,FINITE_BAG_OF_SET] >>
-    `Gi (BAG_INSERT A' (BAG_OF_SET Γ')) A'`
-      by simp[Gi_ax,BAG_IN_BAG_INSERT] >>
-    `Gi (BAG_INSERT (A Imp A') (BAG_OF_SET Γ')) A'`
-      by metis_tac[Gi_limp] >>
-    `Gi ((BAG_OF_SET Γ) ⊎ (BAG_OF_SET Γ')) A'`
-      by metis_tac[Gi_cut] >>
-    `Gi (unibag (BAG_OF_SET Γ ⊎ BAG_OF_SET Γ')) A'` by metis_tac[Gi_unibag] >>
+    `FINITE_BAG (BAG_OF_SET Γ')` by metis_tac[N_FINITE,FINITE_BAG_OF_SET] >>
+    `G (BAG_INSERT A' (BAG_OF_SET Γ')) A'`
+      by simp[G_ax,BAG_IN_BAG_INSERT] >>
+    `G (BAG_INSERT (A Imp A') (BAG_OF_SET Γ')) A'`
+      by metis_tac[G_limp] >>
+    `G ((BAG_OF_SET Γ) ⊎ (BAG_OF_SET Γ')) A'`
+      by metis_tac[G_cut] >>
+    `G (unibag (BAG_OF_SET Γ ⊎ BAG_OF_SET Γ')) A'` by metis_tac[G_unibag] >>
     fs[unibag_UNION])
- >- (rename [`Ni (_ INSERT _) C`] >>
+ >- (rename [`N (_ INSERT _) C`] >>
      fs[BAG_OF_SET_UNION,BAG_OF_SET_INSERT] >>
      qabbrev_tac `Δ = ((BAG_OF_SET Γ) ⊎ (BAG_OF_SET D1) ⊎ (BAG_OF_SET D2))` >>
      `FINITE_BAG (BAG_INSERT A Δ)`
        by (simp[Abbr`Δ`,FINITE_BAG_THM] >>
-           metis_tac[FINITE_BAG_OF_SET,Ni_FINITE,FINITE_INSERT]) >>
-      `Gi (BAG_INSERT A Δ) C`
-        by (`Gi (BAG_MERGE {|A|} Δ) C`
-              suffices_by metis_tac[BAG_MERGE_ELBAG_SUB_BAG_INSERT,Gi_lw] >>
+           metis_tac[FINITE_BAG_OF_SET,N_FINITE,FINITE_INSERT]) >>
+      `G (BAG_INSERT A Δ) C`
+        by (`G (BAG_MERGE {|A|} Δ) C`
+              suffices_by metis_tac[BAG_MERGE_ELBAG_SUB_BAG_INSERT,G_lw] >>
             simp[Abbr`Δ`] >>
-            irule Gi_lw >>
+            irule G_lw >>
             conj_tac >- fs[FINITE_BAG_MERGE,FINITE_BAG_THM] >>
             qexists_tac `BAG_MERGE {|A|} (BAG_OF_SET D1)` >>
             simp[] >>
@@ -384,12 +481,12 @@ Proof
             fs[]) >>
       `FINITE_BAG (BAG_INSERT B Δ)`
       by (simp[Abbr`Δ`,FINITE_BAG_THM] >>
-              metis_tac[FINITE_BAG_OF_SET,Ni_FINITE,FINITE_INSERT]) >>
-      `Gi (BAG_INSERT B Δ) C`
-        by (`Gi (BAG_MERGE {|B|} Δ) C`
-              suffices_by metis_tac[BAG_MERGE_ELBAG_SUB_BAG_INSERT,Gi_lw] >>
+              metis_tac[FINITE_BAG_OF_SET,N_FINITE,FINITE_INSERT]) >>
+      `G (BAG_INSERT B Δ) C`
+        by (`G (BAG_MERGE {|B|} Δ) C`
+              suffices_by metis_tac[BAG_MERGE_ELBAG_SUB_BAG_INSERT,G_lw] >>
             simp[Abbr`Δ`] >>
-            irule Gi_lw >>
+            irule G_lw >>
             conj_tac >- fs[FINITE_BAG_MERGE,FINITE_BAG_THM] >>
             qexists_tac `BAG_MERGE {|B|} (BAG_OF_SET D2)` >>
             simp[] >>
@@ -397,50 +494,50 @@ Proof
                BAG_OF_SET,BAG_UNION,SUB_BAG,BAG_INN,IN_DEF] >>
             rw[] >>
             fs[]) >>
-      `Gi Δ (A Or B)`
+      `G Δ (A Or B)`
         by (simp[Abbr`Δ`] >>
-            irule Gi_lw_BAG_UNION >>
-            conj_tac >- metis_tac[FINITE_INSERT,Ni_FINITE,FINITE_BAG_OF_SET] >>
-            irule Gi_lw_BAG_UNION >>
-            conj_tac >- metis_tac[FINITE_INSERT,Ni_FINITE,FINITE_BAG_OF_SET] >>
+            irule G_lw_BAG_UNION >>
+            conj_tac >- metis_tac[FINITE_INSERT,N_FINITE,FINITE_BAG_OF_SET] >>
+            irule G_lw_BAG_UNION >>
+            conj_tac >- metis_tac[FINITE_INSERT,N_FINITE,FINITE_BAG_OF_SET] >>
             metis_tac[]) >>
-      `Gi (BAG_INSERT (A Or B) Δ) C` by metis_tac[Gi_lor] >>
-      `Gi ((BAG_OF_SET Γ) ⊎ Δ) C` by metis_tac[Gi_cut] >>
-      `Gi (unibag (BAG_OF_SET Γ ⊎ Δ)) C` by metis_tac[Gi_unibag] >>
+      `G (BAG_INSERT (A Or B) Δ) C` by metis_tac[G_lor] >>
+      `G ((BAG_OF_SET Γ) ⊎ Δ) C` by metis_tac[G_cut] >>
+      `G (unibag (BAG_OF_SET Γ ⊎ Δ)) C` by metis_tac[G_unibag] >>
       `(unibag (BAG_OF_SET Γ ⊎ Δ))
         = BAG_MERGE (BAG_MERGE (BAG_OF_SET Γ) (BAG_OF_SET D1)) (BAG_OF_SET D2)`
          suffices_by metis_tac[] >>
       rw[Abbr`Δ`,unibag_UNION,BAG_MERGE,FUN_EQ_THM])
- >- (`Gi {|Bot|} A` by metis_tac[Gi_bot,BAG_IN_BAG_INSERT,FINITE_BAG] >>
-     metis_tac[Gi_cut,BAG_UNION_EMPTY])
+ >- (`G {|Bot|} A` by metis_tac[G_bot,BAG_IN_BAG_INSERT,FINITE_BAG] >>
+     metis_tac[G_cut,BAG_UNION_EMPTY])
 QED
 
-(* Apparently Ni takes a subset here!? *)
-Theorem Gi_Ni:
-  ∀Γ A. Gi Γ A ==> ?Γ'. Γ' ⊆ (SET_OF_BAG Γ) /\ Ni Γ' A
+(* Apparently N takes a subset here!? *)
+Theorem G_N:
+  ∀Γ A. G Γ A ==> ?Γ'. Γ' ⊆ (SET_OF_BAG Γ) /\ N Γ' A
 Proof
-  Induct_on `Gi` >> rw[]
-    >- (qexists_tac `{A}` >> simp[SUBSET_DEF,SET_OF_BAG] >> metis_tac[Ni_ax])
+  Induct_on `G` >> rw[]
+    >- (qexists_tac `{A}` >> simp[SUBSET_DEF,SET_OF_BAG] >> metis_tac[N_ax])
     >- (qexists_tac `{Bot}` >> simp[SUBSET_DEF,SET_OF_BAG] >>
-        metis_tac[Ni_bot,Ni_ax])
+        metis_tac[N_bot,N_ax])
     >- (qexists_tac `Γ'` >> fs[SET_OF_BAG,BAG_UNION,BAG_INSERT])
-    >- (rename [`Ni _ C`] >>
-        `Ni {A And B} (A And B)` by metis_tac[Ni_ax] >>
-        `Ni {A And B} A` by metis_tac[Ni_andel] >>
-        `Ni (Γ' DELETE A) (A Imp C)`
-          by metis_tac[Ni_impi_DELETE] >>
-        `Ni ((Γ' DELETE A) ∪ {A And B}) C` by metis_tac[Ni_impe] >>
-        `Ni ((A And B) INSERT (Γ' DELETE A)) C`
+    >- (rename [`N _ C`] >>
+        `N {A And B} (A And B)` by metis_tac[N_ax] >>
+        `N {A And B} A` by metis_tac[N_andel] >>
+        `N (Γ' DELETE A) (A Imp C)`
+          by metis_tac[N_impi_DELETE] >>
+        `N ((Γ' DELETE A) ∪ {A And B}) C` by metis_tac[N_impe] >>
+        `N ((A And B) INSERT (Γ' DELETE A)) C`
                   by metis_tac[UNION_COMM,INSERT_SING_UNION] >>
         qexists_tac `(A And B) INSERT Γ' DELETE A` >>
         fs[SET_OF_BAG_INSERT] >>
         fs[SUBSET_DEF] >>
         metis_tac[])
-    >- (rename [`Ni _ C`] >>
-        `Ni {A And B} (A And B)` by metis_tac[Ni_ax] >>
-        `Ni {A And B} B` by metis_tac[Ni_ander] >>
-        `Ni (B INSERT Γ') C` by metis_tac[Ni_lw] >>
-        `Ni (Γ' DELETE B) (B Imp C)`
+    >- (rename [`N _ C`] >>
+        `N {A And B} (A And B)` by metis_tac[N_ax] >>
+        `N {A And B} B` by metis_tac[N_ander] >>
+        `N (B INSERT Γ') C` by metis_tac[N_lw] >>
+        `N (Γ' DELETE B) (B Imp C)`
           by (Cases_on `B ∈ Γ'`
               >- (`?Γ0. (Γ' = B INSERT Γ0) /\ B NOTIN Γ0`
                     by metis_tac[DECOMPOSITION] >>
@@ -448,76 +545,76 @@ Proof
                   `(B INSERT Γ0) DELETE B = Γ0`
                     by (dsimp[EXTENSION] >>
                         metis_tac[]) >>
-                  simp[Ni_impi])
-              >- (simp[DELETE_NON_ELEMENT_RWT,Ni_impi])) >>
-        `Ni ((Γ' DELETE B) ∪ {A And B}) C` by metis_tac[Ni_impe] >>
-        `Ni ((A And B) INSERT (Γ' DELETE B)) C`
+                  simp[N_impi])
+              >- (simp[DELETE_NON_ELEMENT_RWT,N_impi])) >>
+        `N ((Γ' DELETE B) ∪ {A And B}) C` by metis_tac[N_impe] >>
+        `N ((A And B) INSERT (Γ' DELETE B)) C`
           by metis_tac[UNION_COMM,INSERT_SING_UNION] >>
         qexists_tac `(A And B) INSERT Γ' DELETE B` >>
         fs[SET_OF_BAG_INSERT] >>
         fs[SUBSET_DEF] >>
         metis_tac[])
     >- (qexists_tac `Γ' ∪ Γ''` >> simp[] >>
-        metis_tac[Ni_andi])
-    >- (rename [`Ni _ C`] >>
+        metis_tac[N_andi])
+    >- (rename [`N _ C`] >>
         qabbrev_tac `Δ = (A Or B) INSERT (SET_OF_BAG Γ)` >>
         fs[SET_OF_BAG_INSERT] >>
-        `FINITE_BAG Γ` by metis_tac[Gi_FINITE,FINITE_BAG_THM] >>
-        `Ni (A INSERT Δ) C`
-          by (irule Ni_lw_SUBSET >>
+        `FINITE_BAG Γ` by metis_tac[G_FINITE,FINITE_BAG_THM] >>
+        `N (A INSERT Δ) C`
+          by (irule N_lw_SUBSET >>
               simp[Abbr`Δ`] >>
               qexists_tac `Γ'` >>
               simp[] >>
               metis_tac[INSERT_COMM,SUBSET_INSERT_RIGHT]) >>
-        `Ni (B INSERT Δ) C`
-          by (irule Ni_lw_SUBSET >>
+        `N (B INSERT Δ) C`
+          by (irule N_lw_SUBSET >>
               simp[Abbr`Δ`] >>
               qexists_tac `Γ''` >>
               simp[] >>
               metis_tac[INSERT_COMM,SUBSET_INSERT_RIGHT]) >>
         qexists_tac `Δ` >>
         simp[] >>
-        `Ni {(A Or B)} (A Or B)` by metis_tac[Ni_ax] >>
+        `N {(A Or B)} (A Or B)` by metis_tac[N_ax] >>
         `FINITE ({A Or B} ∪ (SET_OF_BAG Γ))`
           by (`FINITE (SET_OF_BAG Γ)`
                 by metis_tac[FINITE_SET_OF_BAG] >>
               metis_tac[FINITE_UNION,FINITE_DEF]) >>
-        `Ni ({A Or B} ∪ (SET_OF_BAG Γ)) (A Or B)`
-          by metis_tac[SUBSET_UNION,Ni_lw_SUBSET] >>
-        `Ni Δ (A Or B)`
+        `N ({A Or B} ∪ (SET_OF_BAG Γ)) (A Or B)`
+          by metis_tac[SUBSET_UNION,N_lw_SUBSET] >>
+        `N Δ (A Or B)`
           by (simp[Abbr`Δ`] >>metis_tac[INSERT_SING_UNION]) >>
-        `Ni (Δ ∪ Δ ∪ Δ) C` by metis_tac[Ni_ore] >>
+        `N (Δ ∪ Δ ∪ Δ) C` by metis_tac[N_ore] >>
         metis_tac[UNION_IDEMPOT])
-    >- (qexists_tac `Γ'` >> simp[Ni_orir])
-    >- (qexists_tac `Γ'` >> simp[Ni_oril])
-    >- (rename [`Ni _ C`] >>
+    >- (qexists_tac `Γ'` >> simp[N_orir])
+    >- (qexists_tac `Γ'` >> simp[N_oril])
+    >- (rename [`N _ C`] >>
         fs[SET_OF_BAG_INSERT] >>
-        `FINITE_BAG Γ` by metis_tac[Gi_FINITE,FINITE_BAG_THM] >>
+        `FINITE_BAG Γ` by metis_tac[G_FINITE,FINITE_BAG_THM] >>
         `FINITE (SET_OF_BAG Γ)` by metis_tac[FINITE_SET_OF_BAG] >>
-        `Ni {A Imp B} (A Imp B)` by metis_tac[Ni_ax] >>
-        `Ni (SET_OF_BAG Γ) A` by metis_tac[Ni_lw_SUBSET] >>
-        `Ni ({A Imp B} ∪ (SET_OF_BAG Γ)) B` by metis_tac[Ni_impe] >>
-        `Ni ((A Imp B) INSERT (SET_OF_BAG Γ)) B`
+        `N {A Imp B} (A Imp B)` by metis_tac[N_ax] >>
+        `N (SET_OF_BAG Γ) A` by metis_tac[N_lw_SUBSET] >>
+        `N ({A Imp B} ∪ (SET_OF_BAG Γ)) B` by metis_tac[N_impe] >>
+        `N ((A Imp B) INSERT (SET_OF_BAG Γ)) B`
           by metis_tac[INSERT_SING_UNION] >>
         qexists_tac `(A Imp B) INSERT SET_OF_BAG Γ` >>
         simp[SUBSET_INSERT_RIGHT] >>
-        `Ni (B INSERT (SET_OF_BAG Γ)) C`
-          by metis_tac[Ni_lw_SUBSET,FINITE_INSERT] >>
-        `Ni (SET_OF_BAG Γ) (B Imp C)` by metis_tac[Ni_impi] >>
-        `Ni ((SET_OF_BAG Γ) ∪ ((A Imp B) INSERT SET_OF_BAG Γ)) C`
-          by metis_tac[Ni_impe] >>
+        `N (B INSERT (SET_OF_BAG Γ)) C`
+          by metis_tac[N_lw_SUBSET,FINITE_INSERT] >>
+        `N (SET_OF_BAG Γ) (B Imp C)` by metis_tac[N_impi] >>
+        `N ((SET_OF_BAG Γ) ∪ ((A Imp B) INSERT SET_OF_BAG Γ)) C`
+          by metis_tac[N_impe] >>
         metis_tac[UNION_COMM,UNION_ASSOC,UNION_IDEMPOT,INSERT_SING_UNION])
-    >- (rename [`Ni Δ C`,`Ni _ (A Imp C)`] >>
+    >- (rename [`N Δ C`,`N _ (A Imp C)`] >>
         fs[SET_OF_BAG_INSERT] >>
         `FINITE (A INSERT (SET_OF_BAG Γ))`
-          by (simp[] >> metis_tac[Gi_FINITE,FINITE_BAG_THM]) >>
-        `Ni (A INSERT (SET_OF_BAG Γ)) C` by metis_tac[Ni_lw_SUBSET] >>
-        `Ni (SET_OF_BAG Γ) (A Imp C)` by metis_tac[Ni_impi] >>
+          by (simp[] >> metis_tac[G_FINITE,FINITE_BAG_THM]) >>
+        `N (A INSERT (SET_OF_BAG Γ)) C` by metis_tac[N_lw_SUBSET] >>
+        `N (SET_OF_BAG Γ) (A Imp C)` by metis_tac[N_impi] >>
         metis_tac[SUBSET_REFL])
-    >- (rename [`Gi Γ A`,`Gi (BAG_INSERT A Γ2) B`,`Ni Δ1 A`,`Ni Δ2 B`] >>
-        `Ni (A INSERT Δ2) B` by metis_tac[Ni_lw] >>
-        `Ni (Δ2 DELETE A) (A Imp B)` by metis_tac[Ni_impi_DELETE] >>
-        `Ni ((Δ2 DELETE A) ∪ Δ1) B` by metis_tac[Ni_impe] >>
+    >- (rename [`G Γ A`,`G (BAG_INSERT A Γ2) B`,`N Δ1 A`,`N Δ2 B`] >>
+        `N (A INSERT Δ2) B` by metis_tac[N_lw] >>
+        `N (Δ2 DELETE A) (A Imp B)` by metis_tac[N_impi_DELETE] >>
+        `N ((Δ2 DELETE A) ∪ Δ1) B` by metis_tac[N_impe] >>
         qexists_tac `((Δ2 DELETE A) ∪ Δ1)` >>
         rw[]
           >- (irule SUBSET_TRANS >>
@@ -529,21 +626,22 @@ Proof
               metis_tac[SUBSET_DEF,IN_UNION]))
 QED
 
-Theorem Gi_iff_Ni:
-∀Γ A. Gi Γ A <=> Ni (SET_OF_BAG Γ) A
+Theorem G_iff_N:
+∀Γ A. G Γ A <=> N (SET_OF_BAG Γ) A
 Proof
   rw[] >>
   EQ_TAC
     >- (rw[] >>
-      `?D. D ⊆ (SET_OF_BAG Γ) ∧ Ni D A` by metis_tac[Gi_Ni] >>
-      metis_tac[Ni_lw_SUBSET,Gi_FINITE,FINITE_SET_OF_BAG]) >>
+      `?D. D ⊆ (SET_OF_BAG Γ) ∧ N D A` by metis_tac[G_N] >>
+      metis_tac[N_lw_SUBSET,G_FINITE,FINITE_SET_OF_BAG]) >>
   rw[] >>
-  `Gi (unibag Γ) A` by metis_tac[Ni_Gi] >>
-  metis_tac[Gi_unibag]
+  `G (unibag Γ) A` by metis_tac[N_G] >>
+  metis_tac[G_unibag]
 QED
 
-val _ = set_fixity "Gi" (Infix (NONASSOC, 320));
-val _ = set_fixity "Ni" (Infix (NONASSOC, 320));
+val _ = set_fixity "G" (Infix (NONASSOC, 320));
+val _ = set_fixity "N" (Infix (NONASSOC, 320));
+val _ = set_fixity "Nd" (Infix (NONASSOC, 320));
 val _ = set_fixity "BAG_MERGE" (Infix (NONASSOC, 330));
 (* val _ = set_fixity "BAG_INSERT" (Infixl 330); *)
 
